Auto/Embedding/LamSystem.lean
@@ -1786,8 +1786,8 @@ theorem LamGenModify.rwGenAtIfSign {modify} (H : LamGenModify lval modify weaken
 
 -- Boolean theorems
 def LamTerm.emb : LamTerm := .mkForallEF (.base .bool) (.mkOr
-  (.mkEq (.base .bool) (.bvar 0) (.base .trueb'))
-  (.mkEq (.base .bool) (.bvar 0) (.base .falseb')))
+  (.mkEq (.base .bool) (.bvar 0) (.base .trueb))
+  (.mkEq (.base .bool) (.bvar 0) (.base .falseb)))
 
 def LamWF.emb : LamWF ltv ⟨lctx, LamTerm.emb, .base .prop⟩ :=
   .mkForallEF (.mkOr (.mkEq (.ofBVar 0) (.ofBase .ofTrueB')) (.mkEq (.ofBVar 0) (.ofBase .ofFalseB')))
@@ -1800,7 +1800,7 @@ theorem LamThmValid.emb : LamThmValid lval [] LamTerm.emb := by
     case false => apply Or.inr; rfl
     case true => apply Or.inl; rfl
 
-def LamTerm.false_ne_true : LamTerm := .mkNot (.mkEq (.base .bool) (.base .falseb') (.base .trueb'))
+def LamTerm.false_ne_true : LamTerm := .mkNot (.mkEq (.base .bool) (.base .falseb) (.base .trueb))
 
 def LamWF.false_ne_true : LamWF ltv ⟨lctx, LamTerm.false_ne_true, .base .prop⟩ :=
   .mkNot (.mkEq (.ofBase .ofFalseB') (.ofBase .ofTrueB'))
@@ -1810,7 +1810,7 @@ theorem LamThmValid.false_ne_true : LamThmValid lval [] LamTerm.false_ne_true :=
   intro h; cases h
 
 def LamTerm.not_true_eq_false : LamTerm := .mkEq (.base .bool)
-  (.app (.base .bool) (.base .notb') (.base .trueb')) (.base .falseb')
+  (.app (.base .bool) (.base .notb) (.base .trueb)) (.base .falseb)
 
 def LamWF.not_true_eq_false : LamWF ltv ⟨lctx, LamTerm.not_true_eq_false, .base .prop⟩ :=
   .mkEq (.ofApp _ (.ofBase .ofNotB') (.ofBase .ofTrueB')) (.ofBase .ofFalseB')
@@ -1819,7 +1819,7 @@ theorem LamThmValid.not_true_eq_false : LamThmValid lval [] LamTerm.not_true_eq_
   intro lctx'; rw [pushLCtxs_nil]; exists LamWF.not_true_eq_false; intro _; rfl
 
 def LamTerm.not_false_eq_true : LamTerm := .mkEq (.base .bool)
-  (.app (.base .bool) (.base .notb') (.base .falseb')) (.base .trueb')
+  (.app (.base .bool) (.base .notb) (.base .falseb)) (.base .trueb)
 
 def LamWF.not_false_eq_true : LamWF ltv ⟨lctx, LamTerm.not_false_eq_true, .base .prop⟩ :=
   .mkEq (.ofApp _ (.ofBase .ofNotB') (.ofBase .ofFalseB')) (.ofBase .ofTrueB')
@@ -1828,7 +1828,7 @@ theorem LamThmValid.not_false_eq_true : LamThmValid lval [] LamTerm.not_false_eq
   intro lctx'; rw [pushLCtxs_nil]; exists LamWF.not_false_eq_true; intro _; rfl
 
 def LamTerm.false_and_eq_false : LamTerm := .mkForallEF (.base .bool) (.mkEq (.base .bool)
-  (.app (.base .bool) (.app (.base .bool) (.base .andb') (.base .falseb')) (.bvar 0)) (.base .falseb'))
+  (.app (.base .bool) (.app (.base .bool) (.base .andb) (.base .falseb)) (.bvar 0)) (.base .falseb))
 
 def LamWF.false_and_eq_false : LamWF ltv ⟨lctx, LamTerm.false_and_eq_false, .base .prop⟩ :=
   .mkForallEF (.mkEq (.ofApp _ (.ofApp _ (.ofBase .ofAndB') (.ofBase .ofFalseB')) (.ofBVar 0)) (.ofBase .ofFalseB'))
@@ -1837,7 +1837,7 @@ theorem LamThmValid.false_and_eq_false : LamThmValid lval [] LamTerm.false_and_e
   intro lctx'; rw [pushLCtxs_nil]; exists LamWF.false_and_eq_false; intro _ b; rfl
 
 def LamTerm.true_and_eq_id : LamTerm := .mkForallEF (.base .bool) (.mkEq (.base .bool)
-  (.app (.base .bool) (.app (.base .bool) (.base .andb') (.base .trueb')) (.bvar 0)) (.bvar 0))
+  (.app (.base .bool) (.app (.base .bool) (.base .andb) (.base .trueb)) (.bvar 0)) (.bvar 0))
 
 def LamWF.true_and_eq_id : LamWF ltv ⟨lctx, LamTerm.true_and_eq_id, .base .prop⟩ :=
   .mkForallEF (.mkEq (.ofApp _ (.ofApp _ (.ofBase .ofAndB') (.ofBase .ofTrueB')) (.ofBVar 0)) (.ofBVar 0))
@@ -1846,7 +1846,7 @@ theorem LamThmValid.true_and_eq_id : LamThmValid lval [] LamTerm.true_and_eq_id 
   intro lctx'; rw [pushLCtxs_nil]; exists LamWF.true_and_eq_id; intro _ b; rfl
 
 def LamTerm.false_or_eq_id : LamTerm := .mkForallEF (.base .bool) (.mkEq (.base .bool)
-  (.app (.base .bool) (.app (.base .bool) (.base .orb') (.base .falseb')) (.bvar 0)) (.bvar 0))
+  (.app (.base .bool) (.app (.base .bool) (.base .orb) (.base .falseb)) (.bvar 0)) (.bvar 0))
 
 def LamWF.false_or_eq_id : LamWF ltv ⟨lctx, LamTerm.false_or_eq_id, .base .prop⟩ :=
   .mkForallEF (.mkEq (.ofApp _ (.ofApp _ (.ofBase .ofOrB') (.ofBase .ofFalseB')) (.ofBVar 0)) (.ofBVar 0))
@@ -1855,7 +1855,7 @@ theorem LamThmValid.false_or_eq_id : LamThmValid lval [] LamTerm.false_or_eq_id 
   intro lctx'; rw [pushLCtxs_nil]; exists LamWF.false_or_eq_id; intro _ b; rfl
 
 def LamTerm.true_or_eq_true : LamTerm := .mkForallEF (.base .bool) (.mkEq (.base .bool)
-  (.app (.base .bool) (.app (.base .bool) (.base .orb') (.base .trueb')) (.bvar 0)) (.base .trueb'))
+  (.app (.base .bool) (.app (.base .bool) (.base .orb) (.base .trueb)) (.bvar 0)) (.base .trueb))
 
 def LamWF.true_or_eq_true : LamWF ltv ⟨lctx, LamTerm.true_or_eq_true, .base .prop⟩ :=
   .mkForallEF (.mkEq (.ofApp _ (.ofApp _ (.ofBase .ofOrB') (.ofBase .ofTrueB')) (.ofBVar 0)) (.ofBase .ofTrueB'))
@@ -1864,7 +1864,7 @@ theorem LamThmValid.true_or_eq_true : LamThmValid lval [] LamTerm.true_or_eq_tru
   intro lctx'; rw [pushLCtxs_nil]; exists LamWF.true_or_eq_true; intro _ b; rfl
 
 def LamTerm.ofPropSpec : LamTerm := .mkForallEF (.base .prop) (.mkEq (.base .prop)
-  (.mkEq (.base .bool) (.app (.base .prop) (.base .ofProp') (.bvar 0)) (.base .trueb')) (.bvar 0))
+  (.mkEq (.base .bool) (.app (.base .prop) (.base .ofProp) (.bvar 0)) (.base .trueb)) (.bvar 0))
 
 def LamWF.ofPropSpec : LamWF ltv ⟨lctx, LamTerm.ofPropSpec, .base .prop⟩ :=
   .mkForallEF (.mkEq (.mkEq (.ofApp _ (.ofBase .ofOfProp') (.ofBVar 0)) (.ofBase .ofTrueB')) (.ofBVar 0))
